\documentclass[12pt]{article}

\addtolength{\textwidth}{.6in}
\addtolength{\oddsidemargin}{-.3in}
\setlength{\textheight}{8.4in}
\setlength{\topmargin}{-.25in}
\setlength{\headheight}{0.0in}
\renewcommand{\baselinestretch}{1.0}
\linespread{1.15}

\usepackage{cite}
\usepackage{times, verbatim,xcolor,bm}
\usepackage{amsbsy,amssymb, amsmath, amsthm}
\usepackage{hyperref}

\newtheorem{definition}{Definition}
\newtheorem{theorem}{Theorem}
\newtheorem{lemma}{Lemma}
\newtheorem{corollary}{Corollary}
\newtheorem{assumption}{Assumption}
\newtheorem{fact}{Fact}

\newcommand{\ve}{\varepsilon}
\newcommand{\ov}{\overline}
\newcommand{\un}{\underline}
\newcommand{\ta}{\theta}
\newcommand{\Ta}{\Theta}
\newcommand{\expect}{\mathbb{E}}

\begin{document}
\title{\vskip-0.6in Gradualism Bellman Equation and Value Function}
\author{ECN 490}
\date{\today}
\maketitle

\title{Lobby}
\[
\max_{m^t,l^t} \sum_{t=1}^\infty \beta^{t-1}\left\{A(m_t)F^\alpha\cdot l^{1-\alpha}_t\cdot P^W-l_t-\mu_t
  \right\} \hskip.2in \text{s.t.} \hskip.2in  m_{t+1}=(1-\delta)m_{t}+\mu_t
\]
\begin{center}\text{So} $\mu_t=m_{t+1}-(1-\delta)m_{t}$\end{center}

\title{Bellman Equation}
\[
  V_l(m_t)=\max_{m_t,l_t}\left\{A(m_t)F^\alpha\cdot (l_t)^{1-\alpha}\cdot P^W-l_t-(m_{t+1}-(1-\delta)m_t)+\beta V_l(m_{t+1})
  \right\} \hskip.2in 
\]
\begin{center}\text{In the optimal stage} $m_t=m_t^\ast=m^\ast_{t+1}$\end{center}
\title{Value Function}
\[
  V_l(m_{t+1}^\ast)=\left\{A(m_{t+1}^\ast)F^\alpha\cdot (l^\ast_t)^{1-\alpha}\cdot P^W-l_t^\ast-(m^\ast_{t+1}-(1-\delta)m^\ast_{t+1})+\beta V_l(m^\ast_{t+1})
 \right\} \hskip.2in
\]
\begin{center}\title{Which implies that}\end{center}
\[V_l(m_{t+1}^\ast)=\frac{1}{1-\beta}[A(m_{t+1}^\ast)\cdot F^\alpha\cdot (l^\ast_t)^{1-\alpha}\cdot P^W-\delta(m^\ast_{t+1})]\]
\title{FOCs}

\[\frac{\partial V_l(m_{t+1})}{\partial m_{t+1}}=\frac{1}{1-\beta}\cdot [\frac{\partial A(m_{t+1})}{\partial m_{t+1}}\cdot F^\alpha \cdot l^{1-\alpha}_t \cdot P^W-\delta]=0
\]
\[\frac{\partial V_l}{\partial m_t}=\frac{\partial A(m_t)}{\partial m_t} \cdot F^\alpha \cdot l^{1-\alpha}_t \cdot P^W-\delta+\frac{\beta}{1-\beta}\cdot [\frac{\partial A(m_{t+1})}{\partial m_{t+1}}\cdot F^\alpha \cdot l^{1-\alpha}_t \cdot P^W-\delta]=1
\]
\[
\frac{\partial V_L}{\partial l_t}= (1-\alpha) \cdot A(m_t) \cdot F^\alpha \cdot l^{-\alpha} \cdot P^W =1
\]
\[
t=\text{this period}
\]
\[
t+1=\text{next period}
\]
\[
\beta=\text{discount factor}
\]
\[
\delta=\text{deprecation factor}
\]

\end{document}